CellularAutomatas/proofs/constructions/composition/trace_kx.lean
@@ -1,0 +1,155 @@
+import CellularAutomatas.defs
+import CellularAutomatas.proofs.constructions.speedup_compressed
+namespace CellularAutomatas
+
+open CellAutomaton
+
+structure TraceKx where
+  k: ℕ
+  α: Type
+  β: Type
+  [_inst_α: Alphabet α]
+  [_inst_β: Alphabet β]
+  [inst: NeZero k]
+  C_orig: CellAutomaton α β
+
+attribute [instance] TraceKx.inst
+attribute [instance] TraceKx._inst_α
+attribute [instance] TraceKx._inst_β
+
+namespace TraceKx
+
+  variable (e: TraceKx)
+
+  def C: CellAutomaton e.α (Fin e.k → e.β？) := {
+    Q := Fin (e.k + 1) → e.C_orig.Q
+    δ := fun a b c =>
+      let next_s := e.C_orig.δ (a (Fin.last e.k)) (b (Fin.last e.k)) (c (Fin.last e.k))
+      Fin.snoc (Fin.tail b) next_s
+    embed := fun a =>
+      let s := e.C_orig.embed a
+      fun _ => s
+    project := fun q =>
+      fun i => some (e.C_orig.project (q (i.castSucc)))
+  }
+
+  lemma state_eq (c: Config e.α) (t: ℕ) (p: ℤ) (i: Fin (e.k + 1)):
+      (e.C.nextt ⦋c⦌ t p) i = (e.C_orig.nextt ⦋c⦌ (t + i - e.k) p) := by
+    revert p i
+    induction t with
+    | zero =>
+      intros p i
+      simp [C, CellAutomaton.embed_config]
+      have : (i : ℕ) - e.k = 0 := Nat.sub_eq_zero_of_le (Nat.le_of_lt_succ i.isLt)
+      rw [this]
+      rw [nextt_zero]
+      rfl
+    | succ t ih =>
+      intros p i
+      rw [CellAutomaton.nextt_succ]
+      unfold CellAutomaton.next C
+      simp
+      by_cases h: i = Fin.last e.k
+      · rw [h]
+        simp [Fin.snoc]
+        change e.C_orig.δ (e.C.nextt ⦋c⦌ t (p - 1) (Fin.last e.k)) (e.C.nextt ⦋c⦌ t p (Fin.last e.k)) (e.C.nextt ⦋c⦌ t (p + 1) (Fin.last e.k)) = _
+        rw [ih (p-1) (Fin.last e.k), ih p (Fin.last e.k), ih (p+1) (Fin.last e.k)]
+        simp [CellAutomaton.next]
+      · have h_lt : (i : ℕ) < e.k := by
+          apply Nat.lt_of_le_of_ne
+          · apply Nat.le_of_lt_succ
+            exact i.isLt
+          · intro heq
+            apply h
+            ext
+            simp [heq]
+        have h_cast : i = Fin.castSucc ⟨i, h_lt⟩ := by
+          ext
+          simp
+        rw [h_cast]
+        simp [Fin.snoc, h_lt]
+        change e.C.nextt ⦋c⦌ t p (Fin.succ ⟨i, h_lt⟩) = _
+        rw [ih p (Fin.succ ⟨i, h_lt⟩)]
+        congr 1
+        simp
+        rw [Nat.add_comm (↑i) 1]
+        rw [←Nat.add_assoc]
+
+  theorem spec (c: Config e.α) (t1: ℕ) (p: ℤ):
+      e.C.comp c (t1 + e.k) p =
+        fun (t2: Fin e.k) => some (e.C_orig.comp c (t1 + t2) p)
+      := by
+    unfold CellAutomaton.comp CellAutomaton.project_config
+    simp only [C]
+    simp
+    change (fun (t2 : Fin e.k) => some (e.C_orig.project ((e.C.nextt ⦋c⦌ (t1 + e.k) p) t2.castSucc))) = _
+    funext t2
+    rw [state_eq]
+    congr
+    simp
+    rw [Nat.add_right_comm]
+    rw [Nat.add_sub_cancel]
+
+end TraceKx
+
+structure SpeedupAndTraceKx where
+  k: ℕ
+  α: Type
+  β: Type
+  [_inst_α: Alphabet α]
+  [_inst_β: Alphabet β]
+  [inst: NeZero k]
+  C_orig: CellAutomaton α β
+
+attribute [instance] SpeedupAndTraceKx.inst
+attribute [instance] SpeedupAndTraceKx._inst_α
+attribute [instance] SpeedupAndTraceKx._inst_β
+
+namespace SpeedupAndTraceKx
+
+  variable (e: SpeedupAndTraceKx)
+
+  def T: TraceKx := {
+    k := e.k
+    α := e.α
+    β := e.β
+    C_orig := e.C_orig
+  }
+  example : (CellAutomaton e.α (Fin e.k → e.β？)) := e.T.C
+
+  def SP: SpeedupKx := {
+    k := e.k
+    α := e.α
+    β := Fin e.k → e.β？
+    C_orig := e.T.C
+  }
+  example : (CellAutomaton (Fin e.k → e.α) (Fin e.k → (Fin e.k → e.β？))) := e.SP.C
+
+  def C: CellAutomaton (Fin e.k → e.α) (Fin e.k → e.β) :=
+    e.SP.C.map_project (fun f => fun i => (f 0 i).getD default)
+
+  theorem spec1 {c: Config e.α} {t1: ℕ} {t2: Fin e.k}:
+      e.C.trace (SpeedupKx.compress e.k c) (t1 + 1) t2 = e.C_orig.trace c (e.k * t1 + t2) := by
+    unfold trace
+    have h_comp : ∀ t p, e.C.comp ⦋SpeedupKx.compress e.k c⦌ t p = (fun g i => (g 0 i).getD default) (e.SP.C.comp ⦋SpeedupKx.compress e.k c⦌ t p) := by
+      intros t p
+      unfold CellAutomaton.comp CellAutomaton.project_config
+      simp [C]
+      rfl
+    rw [h_comp]
+    have h_spec : e.SP.C.comp ⦋SpeedupKx.compress e.k c⦌ (t1 + 1) = SpeedupKx.compress e.k (e.T.C.comp c (e.k * (t1 + 1))) := by
+      convert e.SP.spec (t1 + 1)
+    rw [h_spec]
+    unfold SpeedupKx.compress
+    simp only
+    rw [mul_add, mul_one]
+    have h_spec_T : e.T.C.comp c (e.k * t1 + e.k) 0 = fun (t2 : Fin e.k) => some (e.C_orig.comp c (e.k * t1 + t2) 0) := by
+      convert e.T.spec c (e.k * t1) 0
+    simp only [zero_mul, zero_add]
+    erw [h_spec_T]
+    simp
+
+
+end SpeedupAndTraceKx
+
+end CellularAutomatas
